algebra/rg-algebra/AbstractAtomicTest/Specification.thy
@@ -295,6 +295,8 @@ proof -
   finally show ?thesis using fiter_induct_nil by simp
 qed
 
+
+
 end
 
 
@@ -483,5 +485,7 @@ qed
 end
 
 *) 
+
+
 
 end
